# Multipliers & multiplier effects

Consider the case of a close economy:  
$y = C + I + G$
> $y$ - GDP in market prices  
> $C$ - consumption  
> $C = C_0 + c*y^D$  
>> $C_0$ - autonomous consumption (expenditure made for goods and services that cover basic needs)  
>> $c$ - marginal propensity to consume $c = \dfrac{\Delta c}{\Delta y^D}$  
>> $y^D$ - disposable income, $y^D = y - T + Tr$  
>>> $T = T_0 + t*y$  
>>> $T$ - taxes  
>>> $T_0$ - autonomous tax  

## Types of variables:
1. exogenous variables (predetermined/given):  
   - $I$, $G$, $Tr$, $C_0$, $T_0$  
2. Endogenous variables (determined by the model):  
   - $y$, $c$, $y^D$, $T$  

A multiplier shows the impact of a change in 1 variable (that is exogenous) on another variable (that is endogenous) $\Rightarrow$ a formula  
The multiplier effect shows the change $\Rightarrow$ a value that we calculate using a formula  

Steps:
We write the <ins>reduced</ins> form of the model  
$y = C_0 + c * (y - T_0 - t * y + Tr) + I + G$  
$y = C_0 - c * T_0 + c * Tr + I + G + c(1 - t) * y$  
$(1 - c(1-t))y=C_0-cT_0+cTr+I+G$  
$y = \dfrac{1}{1-c(1-t)}*(C_0 - c*T_0+C*Tr+I+G$ - reduced form of the model  

1. Variation in output: (y)  
   1. assume a change in government spending $G$  
$\Delta y = \dfrac{1}{1-c(1-t)}*\Delta G$  
$\alpha _G = \dfrac{\Delta y}{\Delta G} = \dfrac{1}{1-c(1-t)} \Rightarrow$ gov spending multiplier  
    2. assume a change in investment $I$  
$\Delta y = \dfrac{1}{1-c(1-t)} * \Delta I \Rightarrow \alpha _I = \dfrac{\Delta y}{\Delta I} = \alpha _G \Rightarrow$ investment multiplier  
    3. assume a change in autonomous consumption $C_0$  
        $\Delta y = \dfrac{1}{1-c(1-t)} * \Delta C_0$  
        $\alpha _{C_0} = \dfrac{\Delta y}{\Delta C_0} = \alpha _g \Rightarrow$ autonomous consumption multiplier  
    4. assume a change in out. taxes $T_0$  
        $\Delta y = \dfrac{1}{1-c(1-t)} * (-c) * \Delta T_0$  
        $\alpha _{T_0} = \dfrac{\Delta y}{\Delta T_0} = -c * \alpha _G \Rightarrow$ autonomous tax multiplier  
    5. assume a change in transfers $Tr$  
        $\Delta y = \dfrac{1}{1-c(1-t)} * (c) * \Delta Tr$  
        $\alpha _{Tr} = \dfrac{\Delta y}{\Delta Tr} = C * \alpha _G \Rightarrow$ transfers multiplier  
    6. assume a change in the tax rate  
        $y_1 = \dfrac{1}{1-c(1-t_1)}*()$  
        $y_0 = \dfrac{1}{1-c(1-t_0)}*()$  
        $\Delta y = y_1 - y_0 = \dfrac{1}{1-c(1-y_1)} *() - \dfrac{1}{1-c(1-t_0)}*()$  
        > Actually $\dfrac{1}{1-c(1-t_0)} * () is y_0$  

        $\Delta y = \dfrac{1-c(1-t0)-1+c(1-t1)}{(1-c(1-t1))(1-c(1-t0))}$  
        $\Delta y = \dfrac{-c*t_1+c*t_0}{1-c(1-t_1)}*y_0$  
        $\Delta y = \dfrac{-c * \Delta t}{1-c(1-t_1)} * y_0$  
        $\alpha _t = \dfrac{\Delta y}{\Delta t} = \dfrac{-c*y_0}{1-c(1-t_1)} \Rightarrow$ tax rate multiplier  
        > In some textbooks we find $\alpha _t = \dfrac{-c*y_0}{1-c(1-t_0)}$ (because the difference is not too big)

2. Variation in disposable income $y^D$  
   the extended formula for $y^D$:
   $y^D = y - T_0 - t*y +Tr$  
   $y^D = (1-t)y-T_0+Tr$ (extended formula)  
   $y^D=(1-t) * \Delta y - \Delta T_0 + \Delta Tr$ (variation of extended formula)
      1. assume a change in government spending $G$  
        $\Delta y^D = (1-t) * \Delta y$  
        $\Delta y^D = (1-t)$  
        $\frac{\Delta y}{\Delta G} = \alpha _G \Rightarrow \Delta y = \alpha _G * \Delta G$  
        $m * \Delta y^D_G = \frac{\Delta y^D}{\Delta G} = (1-t) * \alpha _G$  
    2. assume a change in investment $I$  
        $\Delta y^D = (1-t) * \Delta y$  
        $\Delta y^D = (1-t) * \alpha _I * \Delta I \Rightarrow m*\Delta y^D_G = \frac{\Delta y^D}{\Delta I} = (1-t) * \alpha _G$  
        > We know that $\alpha _I = \alpha _G$  
    3. assume a change in transfers $Tr$
        $\Delta y^D = (1-t)*\Delta y + \Delta Tr$
        > we know from 1.1. that $\Delta y^D = \frac{1}{1-c(1-t)} * c * \Delta Tr$
        $\Rightarrow \Delta y^D = \frac{(1-t) * c * \Delta Tr}{1-c(1-t)} + \Delta Tr$
        $\frac{(1-t)*c * \Delta Tr + (1-c(1-t)) * \Delta Tr}{1-c(1-t)} = \frac{\Delta Tr((1-t)c+1-c(1-t))}{1-c(1-t)} = \frac{\Delta Tr}{1-c(1-t)} = \Delta Tr * \alpha _G$
        $m*\Delta y^D_Tr = \frac{\Delta y^D}{\Delta Tr} = \alpha _G$
    4. assume a change in T_0
        $\Delta y^D = (1-t)*\Delta y - \Delta T_0$
        > we know from 1.4. that $\Delta y = -c * \alpha * \Delta T$

        $\Delta y^D = (1-t)(-c*\alpha _G * \Delta T_0) - \Delta T_0$
        $\Delta y^D = (\frac{-c(1-t)}{1-c(1-t)}-1)* \Delta T_0$
        $\Delta y^D = \frac{-c(1-t)-1+c(1-t)}{1-c(1-t)} * \Delta T_0$
        $\Delta y^D = -\alpha _G * \Delta T_0 \Rightarrow m\Delta y^D_{T_0} = \frac{\Delta y^D}{\Delta T_0} = - \alpha _G$
    5. assume a change in tax rate $t$
        $y^D_1 = (1-t_1) * y_1 - T_0 + Tr$
        $y^D_0 = (1-t_0) * y_0 - T_0 + Tr$
        $\Delta y^D = y^D_1-y^D_0 = (1-t_1)y_1-(1-t_0)y_0$
        $\Delta y^D = y_1 - t_1*y_1 - y_0+t_0*y_0$
        $\Delta y^D = \Delta y - t_1*y_1 +t_0y_0$
        > Note: $y_1*\Delta t - t_0*\Delta y = t_1*y_1 + t_0*y_0$ thus $\Delta y^D = \Delta y + y_1 * \Delta t - t_0 * \Delta y$
        $\Delta y^D = (1-t_0) * \Delta y + y_1*\Delta t$
    1.6. idfk de ce a facut asta acum
        $\Delta y^D = \frac{-c * \Delta t}{1-c(1-t_1)}$
        $\Delta y^D = (1-t_0)(\frac{-c * \Delta t}{1-c(1-t_1))} + y_1 * \Delta t$
        $m * \Delta y^D_t = \frac{\Delta y^D}{\Delta t} = \frac{-c(1-t_0)}{1-c(1-t_1)} + y_1$
3. variation in budget deficit $BD$:  
$BD = G - T + Tr + Sv$  
$\Delta BD = \Delta G - \Delta T + \Delta Tr + \Delta Sv$
$T=T_0+t*y$
$\Delta T = \Delta T_0 + t * \Delta y$ (except for changes in t)
    1. assume a change in government spending $G$
        $\Delta BD = \Delta G - \Delta T_0 - t * \Delta y + \Delta Tr + \Delta Sv$
        $\Delta BD = \Delta G - t * \Delta y$
        $\Delta y = \alpha _G * \Delta G$
        $\Delta BD = \Delta G - t * \alpha _G * \Delta G$
        $\Delta BD = (1-t * \alpha _G) * \Delta G$
        $m BD_G = \frac{\Delta BD}{\Delta G} = 1 - t * \alpha _G$
    2. assume a change in transfers $Tr$
        $\Delta BD = \Delta G - \Delta T_0 - t \Delta y + \Delta Tr + \Delta Sv$
        $\Delta BD = -t \Delta y + \Delta Tr$
        $\Delta y = c \alpha _G \Delta Tr$
        $\Delta BD = -t * c * \alpha _G * \Delta Tr + \Delta Tr$
        $mBD_{Tr} = \frac{\Delta BD}{\Delta Tr} = 1-t*c*\alpha _G$





4 equations:
$y = C + I + G$
$c = C_0 + c*y^D$
$y^D = y - T + TR$
$T + T_0 + t * y$
which we use on the extended formula to see which changes for the first 3